\subsection{Senkrechte Polarisation}
\input{Figures/senk_Polarisation_copy.tex}

\begin{itemize}
    \item magnetischer/elektrischer Reflexionsfaktor $[1]$
    \item magnetischer Transmissionsfaktor $[1]$
    \item elektrischer Transmissionsfaktor $[1]$
\end{itemize}

\[ \boxed{\texttt{mit } Z_{F0} = 120\pi \approx 377\si{\ohm}} \]
\begin{align*}
    Z_{Fn}                & = Z_{F0}\cdot\frac{1}{\sqrt{\varepsilon_{rn}}}            \\
    \frac{Z_{F1}}{Z_{F2}} & = \frac{\sqrt{\varepsilon_{r2}}}{\sqrt{\varepsilon_{r1}}}
\end{align*}
\[ n: \texttt{Brechungsindex} \quad ; \quad \theta_h = \theta_r\]
\begin{align*}
    \frac{\sin\theta_t}{\sin\theta_h} & = \frac{\lambda_2}{\lambda_1}= \frac{\beta_1}{\beta_2}= \frac{n_1}{n_2} \\
    \sin\theta_t                      & = \sqrt{\frac{\varepsilon_{r1}}{\varepsilon_{r2}}}\cdot \sin\theta_h
\end{align*}
\begin{align*}
    r_s     & =  r_{e s} = r_{m s} =                                                                                                                                          \\
            & = \frac{Z_{F 2} \cdot \cos \theta_h-Z_{F 1} \cdot \cos \theta_t}{Z_{F 2} \cdot \cos \theta_h+Z_{F 1} \cdot \cos \theta_t}                                       \\
            & = \frac{\cos\theta_h-\sqrt{^{\varepsilon_{r2}}/_{\varepsilon_{r1}}-\sin^2\theta_h}}{\cos\theta_h+\sqrt{^{\varepsilon_{r2}}/_{\varepsilon_{r1}}-\sin^2\theta_h}} \\
    t_{m s} & = Z_{F 1} \cdot \frac{2 \cdot \cos \theta_h}{Z_{F 2} \cdot \cos \theta_h+Z_{F 1} \cdot \cos \theta_t}                                                           \\
            & = (1 - r_{s}) \cdot \dfrac{\cos \theta_h}{\cos \theta_t}                                                                                                        \\
            & = \frac{Z_{F1}}{Z_{F2}}\cdot t_{es}                                                                                                                             \\
    t_{e s} & = Z_{F 2} \cdot \frac{2 \cdot \cos \theta_h}{Z_{F 2} \cdot \cos \theta_h+Z_{F 1} \cdot \cos \theta_t}                                                           \\
            & = 1+r_{s}
\end{align*}
\begin{align*}
    E_{r} & = r_{s} \cdot E_{h}   \\
    E_{t} & = t_{e s} \cdot E_{h} \\
    H_{r} & = r_{s} \cdot H_{h}   \\
    H_{t} & = t_{m s} \cdot H_{h}
\end{align*}

\subsection{Parallel Polarisation}
\input{Figures/para_Polaristion_copy.tex}

\begin{itemize}
    \item magnetischer/elektrischer Reflexionsfaktor $[1]$
    \item magnetischer Transmissionsfaktor $[1]$
    \item elektrischer Transmissionsfaktor $[1]$
\end{itemize}

\[ \boxed{\texttt{mit } Z_{F0} = 120\pi \approx 377\si{\ohm}} \]
\begin{align*}
    Z_{Fn}                & = Z_{F0}\cdot\frac{1}{\sqrt{\varepsilon_{rn}}}            \\
    \frac{Z_{F1}}{Z_{F2}} & = \frac{\sqrt{\varepsilon_{r2}}}{\sqrt{\varepsilon_{r1}}}
\end{align*}
\[ n: \texttt{Brechungsindex} \quad ; \quad \theta_h = \theta_r\]
\begin{align*}
    \frac{\sin\theta_t}{\sin\theta_h} & = \frac{\lambda_2}{\lambda_1}= \frac{\beta_1}{\beta_2}= \frac{n_1}{n_2} \\
    \sin\theta_t                      & = \sqrt{\frac{\varepsilon_{r1}}{\varepsilon_{r2}}}\cdot\sin\theta_h
\end{align*}
\begin{align*}
    r_p     & =  r_{e p} = r_{m p} =                                                                                                                                                                                                      \\
            & = \frac{Z_{F 2} \cdot \cos \theta_t-Z_{F 1} \cdot \cos \theta_h}{Z_{F 2} \cdot \cos \theta_t+Z_{F 1} \cdot \cos \theta_h} =                                                                                                 \\
            & = \frac{\varepsilon_{r2}\cos\theta_h-\sqrt{\varepsilon_{r2}\varepsilon_{r1}-{\varepsilon_{r1}}^2\sin^2\theta_h}}{\varepsilon_{r2}\cos\theta_h+\sqrt{{\varepsilon_{r2}\varepsilon_{r1}-{\varepsilon_{r1}}^2\sin^2\theta_h}}} \\
    t_{e p} & = Z_{F 2} \cdot \frac{2 \cdot \cos \theta_h}{Z_{F 1} \cdot \cos \theta_h+Z_{F 2} \cdot \cos \theta_t}                                                                                                                       \\
            & = (1 + r_{p}) \cdot \dfrac{\cos \theta_h}{\cos \theta_t}                                                                                                                                                                    \\
            & = \frac{Z_{F2}}{Z_{F1}}\cdot t_{mp}                                                                                                                                                                                         \\
    t_{m p} & = Z_{F 1} \cdot \frac{2 \cdot \cos \theta_h}{Z_{F 1} \cdot \cos \theta_h+Z_{F 2} \cdot \cos \theta_t}                                                                                                                       \\
            & = 1+r_{p}
\end{align*}
\begin{align*}
    E_{r} & = r_{s} \cdot E_{h}   \\
    E_{t} & = t_{e s} \cdot E_{h} \\
    H_{r} & = r_{s} \cdot H_{h}   \\
    H_{t} & = t_{m s} \cdot H_{h} \\
\end{align*}
